Main: adding --locate, --locate_lib, --locate_ocaml

src/basic/FStar.Options.fst
@@ -269,6 +269,9 @@ let defaults =
       ("query_stats"                  , Bool false);
       ("read_checked_file"            , Unset);
       ("list_plugins"                 , Bool false);
+      ("locate"                       , Bool false);
+      ("locate_lib"                   , Bool false);
+      ("locate_ocaml"                 , Bool false);
       ("read_krml_file"               , Unset);
       ("record_hints"                 , Bool false);
       ("record_options"               , Bool false);
@@ -526,6 +529,9 @@ let get_query_stats             ()      = lookup_opt "query_stats"              
 let get_read_checked_file       ()      = lookup_opt "read_checked_file"        (as_option as_string)
 let get_read_krml_file          ()      = lookup_opt "read_krml_file"           (as_option as_string)
 let get_list_plugins            ()      = lookup_opt "list_plugins"             as_bool
+let get_locate                  ()      = lookup_opt "locate"                   as_bool
+let get_locate_lib              ()      = lookup_opt "locate_lib"               as_bool
+let get_locate_ocaml            ()      = lookup_opt "locate_ocaml"             as_bool
 let get_record_hints            ()      = lookup_opt "record_hints"             as_bool
 let get_record_options          ()      = lookup_opt "record_options"           as_bool
 let get_retry                   ()      = lookup_opt "retry"                    as_bool
@@ -1589,6 +1595,18 @@ let rec specs_with_types warn_unsafe : list (char & string & opt_type & Pprint.d
     "list_plugins",
      Const (Bool true),
     text "List all registered plugins and exit");
+  ( noshort,
+    "locate",
+     Const (Bool true),
+    text "Print the root of the F* installation and exit");
+  ( noshort,
+    "locate_lib",
+    Const (Bool true),
+    text "Print the root of the F* library and exit");
+  ( noshort,
+    "locate_ocaml",
+    Const (Bool true),
+    text "Print the root of the built OCaml F* library and exit");
   ]
 
 and specs (warn_unsafe:bool) : list (FStar.Getopt.opt & Pprint.document) =
@@ -2083,6 +2101,9 @@ let query_cache                  () = get_query_cache                 ()
 let query_stats                  () = get_query_stats                 ()
 let read_checked_file            () = get_read_checked_file           ()
 let list_plugins                 () = get_list_plugins                ()
+let locate                       () = get_locate                      ()
+let locate_lib                   () = get_locate_lib                  ()
+let locate_ocaml                 () = get_locate_ocaml                ()
 let read_krml_file               () = get_read_krml_file              ()
 let record_hints                 () = get_record_hints                ()
 let record_options               () = get_record_options              ()
